\documentclass[titlepage, letterpaper, fleqn]{article}
\usepackage[utf8]{inputenc}
\usepackage{fancyhdr} % fancy headers, of course!
\usepackage{amsmath} % what do you think?
\usepackage{amsthm} % theorems!
\usepackage{extramarks} % more cute things
\usepackage{enumitem} % i'm not sure...
\usepackage{multicol} % multicolumn...?
\usepackage{amssymb} % more symbols
\usepackage{booktabs} % cool looking tables
\usepackage{tikz} %venn and shizzle
\usepackage{lipsum} %lorem ipsum dolor sit amet f u

\topmargin=-0.45in
\evensidemargin=0in
\oddsidemargin=0in
\textwidth=6.5in
\textheight=9.0in
\headsep=0.25in


%
% You should change this things~
%

\newcommand{\mahteacher}{Dr. Viacheslav Kalashnikov}
\newcommand{\mahclass}{Applied Mathematics}
\newcommand{\mahtitle}{Activities 13, 14 \& 15}
\newcommand{\mahdate}{September 7, 2016}
\newcommand{\spacepls}{\vspace{5mm}}
\renewcommand\qedsymbol{\(\blacksquare\)}

%
% Header markings
%

\pagestyle{fancy}
\lhead{1170065 - Xavier Sánchez}
\chead{}
\rhead{}
\lfoot{}
\rfoot{}


\renewcommand\headrulewidth{0.4pt}
\renewcommand\footrulewidth{0.4pt}

\setlength\parindent{0pt}


%
% Create Problem Sections (stolen directly from jdavis/latex-homework-template @ github!)
%

\newcommand{\enterProblemHeader}[1]{
\nobreak\extramarks{}{Problem \arabic{#1} continued on next page\ldots}\nobreak{}
\nobreak\extramarks{Problem \arabic{#1} (continued)}{Problem \arabic{#1} continued on next page\ldots}\nobreak{}
}

\newcommand{\exitProblemHeader}[1]{
\nobreak\extramarks{Problem \arabic{#1} (continued)}{Problem \arabic{#1} continued on next page\ldots}\nobreak{}
\stepcounter{#1}
\nobreak\extramarks{Problem \arabic{#1}}{}\nobreak{}
}

\setcounter{secnumdepth}{0}
\newcounter{partCounter}
\newcounter{homeworkProblemCounter}
\setcounter{homeworkProblemCounter}{1}
\nobreak\extramarks{Exercise \arabic{homeworkProblemCounter}}{}\nobreak{}

% Alias for the Solution section header
\newcommand{\solution}{\textbf{\Large Solution}}

%Alias for the new step section
\newcommand{\steppy}[1]{\textbf{\large #1}}

%
% Homework Problem Environment
%
% This environment takes an optional argument. When given, it will adjust the
% problem counter. This is useful for when the problems given for your
% assignment aren't sequential. See the last 3 problems of this template for an
% example.
%
\newenvironment{homeworkProblem}[1][-1]{
\ifnum#1>0
\setcounter{homeworkProblemCounter}{#1}
\fi
\section{Exercise \arabic{homeworkProblemCounter}}
\setcounter{partCounter}{1}
\enterProblemHeader{homeworkProblemCounter}
}{
\exitProblemHeader{homeworkProblemCounter}
}

%
% Venn diagrams defs
%

% \def\firstcircle{(0,0) circle (1.5cm)}
% \def\secondcircle{(0:2cm) circle (1.5cm)}
% \colorlet{circle edge}{blue!50}
% \colorlet{circle area}{blue!20}

% \tikzset{filled/.style={fill=circle area, draw=circle edge, thick},
%     outline/.style={draw=circle edge, thick}}

%
% My actual info
%

\title{
\vspace{1in}
\textbf{Tecnológico de Monterrey} \\
\vspace{0.5in}
\textmd{\mahclass} \\
\large{\textit{\mahteacher}} \\
\vspace{0.5in}
\textsc{\mahtitle}\\
\textsc{1.4.1: Proof by simple induction}\\
\textsc{1.4.2: Definition by simple recursion}\\
\textsc{1.4.3: Proof by cumulative induction}\\
\author{01170065  - MIT \\
Xavier Fernando Cuauhtémoc Sánchez Díaz \\
\texttt{xavier.sanchezdz@gmail.com}}
\date{\mahdate}
}

\begin{document}

\begin{titlepage}
\maketitle
\end{titlepage}

%
% Actual document starts here~
%

\section{Exercise 1.4.1}

{\large \textbf{a)} Use simple induction to show that for every positive integer \(n\), \(5^n - 1\) is divisible by 4.}

\begin{proof}
1. Basis \\
\[5 ^1 - 1 = 5 - 1 = 4 \tag*{n = 1}\]
2. Induction hypothesis \\
\begin{align*}
& 5^k - 1 \text{ is divisible by 4} \tag*{n=k}\\
& 5^k - 1 = 4m, m \in \mathbb*{N}\\
& 5^k = 4m + 1 \tag*{arithmetic}
\end{align*}
3. Induction step, for \(k = k+1\) \\
\begin{align*}
5^{k+1} - 1 & = \\
& = 5 \cdot 5^k - 1 \\
& = 5(4m + 1) - 1 \tag*{substitution with hypothesis}\\
& = 20m + 5 - 1\\
& = 20m + 4\\
& = 4(5m+1)
\end{align*}
Therefore, \(5^{k+1}-1 = 4(5m+1)\), and thus is divisible by 4.
\end{proof}

\spacepls

{\large \textbf{b)} Use simple induction to show that for every positive integer \(n\), \(n^3 - n\) is divisible by 3.}
%Hint: in the induction step, you will need to make use of the arithmetic fact that (k + 1)^3 = k^3 +3k^2 + 3k + 1.

\begin{proof}
1. Basis \\
\[1^3 - 1 = 1 - 1 = 0 \tag*{n=1}\]
2. Induction hypothesis\\
\begin{align*}
& k^3 - k \text{ is divisible by 3} \tag{n=k} \\
& k^3 - k = 3m, m \in \mathbb{N}
\end{align*}
3. Induction step, for \(k + k+1\) \\
\begin{align*}
(k+1)^3 - (k+1) & = \\
& = k^3 + 3k^2 + 3k + 1 - (k + 1)\tag *{arithmetic} \\
& = k^3 + 3k^2 + 3k - k \tag*{ditto}\\
& = (k^3 - k) + 3k^2 + 3k \tag*{reordering}\\
& = 3m + 3k^2 + 3k \tag*{substitution by hypothesis}\\
& = 3(m + k^2 + k) \tag*{arithmetic}
\end{align*}
Therefore, \(\exists m \in \mathbb{N}\) such that \(k+1\) is divisible by 3, so \(\forall n \in \mathbb{N}, n^3 - n\) is divisible by 3.
\end{proof}

\pagebreak

{\large \textbf{c)} Show by simple induction that for every natural number \(n\), \(\sum \{2^i \colon 0 \leq i \leq n\} = 2^{n+1} - 1\).}

\begin{proof}
1. Basis, with \(n = 1\) \\
\begin{align*}
& 2^{(1 + 1)} - 1 = 2^2 -1 = 4 - 1 = 3 \tag*{RHS}\\
& 2^0 + 2^1 = 1 + 2 = 3 \tag*{LHS}\\
\end{align*}
2. Induction hypothesis\\
\[2^{k+1}-1 = 2^0 + 2^1 + \dots + 2^k \tag*{n=k}\]
3. Induction step, for \(k = k + 1\)\\
\begin{align*}
& 2^{(k+1)+1} -1 =\\
& = 2^{k+2} - 1\\
& = 2 \cdot 2^{k+1} -1\\
& = 2(2^{k+1} - 1) -1 + 2\tag*{modifications to match hypothesis}\\ 
& = 2(2^{k+1} - 1) + 1 \tag*{arithmetic}\\
& = 2(2^0 + 2^1 + \dots + 2^k) + 1 \tag*{substitution by hypothesis}\\
& = 2^1 + 2^2 + \dots + 2^{k+1} + 1 \tag*{ditto}\\
& = 2^0 + 2^1 + 2^2 + \dots + 2^{k+1} \tag*{substitute 1 by \(2^0\)}
\end{align*}
Therefore, \(2^{(k+1)+1} -1 = 2^0 + 2^1 + \dots + 2^{k+1}\)
\end{proof}

\section{Exercise 1.4.2}

{\large \textbf{a)} Let \(f \colon \mathbb{N} \to \mathbb{N}\) be the function defined by putting \(f(0) = 0\) and \(f(n+1) = n\) for all \(n \in \mathbb{N}\).}\\
\textbf{i)} Evaluate this function bottom-up for all arguments 0-5.


\begin{align*}
f(0) = 0\\
f(0+1) = f(1) = 0\\
f(1+1) = f(2) = 1\\
f(2+1) = f(3) = 2\\
f(3+1) = f(4) = 3\\
f(4+1) = f(5) = 4\\
f(5+1) = f(6) = 5\\
\end{align*}

\spacepls

\textbf{ii)} Explain what \(f\) does by expressing it in explicit terms (i.e. without a recursion).

\[f(n) =
\begin{cases}
& n -1 \colon n \in \mathbb{N}, n > 0 \\
& 0, n = 0
\end{cases}
\]

\pagebreak

{\large \textbf{b)} Let \(f \colon \mathbb{N}^+ \to \mathbb{N}\) be  the function that takes each positive integer \(n\) to the greatest natural number \(p\) with \(2^p \leq n\). Define this function by a simple recursion.}
%hint: You will need to divide the recursion step into two cases.

1. Basis: \(f(1) = 0\).

\[f(n+1) =
\begin{cases}
\log_2 (n+1), \log_2 (n+1) \in \mathbb{N}\\
f(n), \log_2 (n+1) \not \in \mathbb{N}
\end{cases}
\]

{\large \textbf{c)} Let \(g \colon \mathbb{N} \times \mathbb{N} \to \mathbb{N}\) be defined by putting \(g(m,0) = m\) for all \(m \in \mathbb{N}\) and \(g(m,n+1) = f(g(m,n))\) where \(f\) is defined in the previous part of this exercise.}\\
\textbf{i)} Evaluate \(g(3,4)\) top-down.

\begin{align*}
g(3,4) & = f(g(3,3)) \\
& = f(f(g(3,2)))\\
& = f(f(f(g(3,1))))\\
& = f(f(f(f(g(3,0)))))\\
& = f(f(f(f(3))))\\
& = f(f(f(2)))\\
& = f(f(1))\\
& = f(0)\\
& = 0
\end{align*}
\spacepls

\textbf{ii)} Explain what \(f\) does by expressing it in explicit terms.

\[f(n) =
\begin{cases}
n - 1 \colon n \in \mathbb{N}, n > 0\\
0, n = 0
\end{cases}
\]

\section{Exercise 1.4.3}

{\large \textbf{a)} Use cumulative induction to show that any postage cost of four or more pence can be covered by two-pence and five-pence stamps.}

\begin{proof}
Let \(j\) be any cost of four or more pence.\\
1. Basis\\
\[4 = (2)(\$2) + (0)(\$5)\]
\[4 = (n)(\$2) + (m)(\$5)\]
2. Inductive step\\
Let \(k\) be any natural number greater than \(j\) that has this property.\\
Since \(n\$2\) covers all even numbers, then just odd numbers remain.\\
And since \(n\$2\) is even, and \(m\$5\) is odd for all \(m\) that are odd,\\
then a combination of \(n\$2\) and \(m\$5\) covers any number \(4 \leq j < k\) such that \(k\).
\end{proof}

\pagebreak

{\large \textbf{b)} Use cumulative induction to show that for every natural number \(n, F(n) \leq 2^n - 1\), where \(F\) is the Fibonacci function.}

\begin{proof}
1. Basis\\
\begin{align*}
F(3) \leq 2^3 -1\\
2 \leq 8 - 1\\
2 \leq 7
\end{align*}
2. Induction step\\
Since \(F(a)\) can be expressed as \(F(a-1) + F(a-2)\), then \(F(a) > f(a-1)\) and \(F(a) > F(a-2)\).\\
Now assume \(F(a +2) = F(j)\),\\
then \(F(j)\) > \(F(a)\) and thus \(j > a\).\\
So \(2^j > 2^a\), and so is \(2^j -1 > 2^a -1\).\\
Therefore, there is a number \(k > j > a\) for which this property holds.
\end{proof}

\spacepls

{\large \textbf{c)} Calculate \(F(5)\) top-down, and then again bottom-up, where again \(F\) is the Fibonacci function.}

\begin{proof}
\begin{align*}
F(5) &= F(4) + F(3)\\
& = F(3) + F(2) + F(2) + F(1)\\
& = F(2) + F(1) + F(1) + F(0) + F(1) + F(0) + F(1)
& = F(1) + F(0) + F(1) + F(1) + F(0) + F(1) + F(0) + F(1)
& = 1 + 0 + 1 + 1 + 0 + 1 + 0 + 1
& = 5
\end{align*}

\begin{align*}
F(0) &= 0\\
F(1) &= 1\\
F(2) &= F(1) + F(0) = 1 + 0 = 1\\
F(3) &= F(2) + F(1) = 1 + 1 = 2\\
F(4) &= F(3) + F(2) = 2 + 1 = 3\\
F(5) &= F(4) + F(3) = 3 + 2 = 5
\end{align*}
\end{proof}

\spacepls

{\large \textbf{d)} Express each of the numbers 14, 15 and 16 as a sum of 3s and/or 8s. Using this fact in your basis, show by cumulative induction that every positive integer \(n \geq 14\) may be expressed as a sum of 3s and/or 8s}.

\begin{proof}
1. Basis\\
\begin{align*}
14 = 3 + 3 + 8\\
15 = 3 + 3 + 3 + 3 + 3\\
16 = 8 + 8
\end{align*}
2. Induction step\\
Let \(j\) be any natural number greater than 14, and \(k\) be any natural number greater than \(j\). And assume \(j\) has this property shown on the basis.\\
Since 14 can be expressed as the sum of 3 and 8, all numbers which can be obtained adding 3s or 8s (i.e. 17 = 14 + 3, or 22 = 14 + 8) can be expressed in the same way.\\
The same follows for all multiples of 3 and 8 (like  15, or 16).\\
And since we only have three cases in succession, then the following \(n \in \mathbb{N}\) is in the first case again.
\end{proof}

\spacepls

{\large \textbf{e)} Show by induction that for every natural number \(n, A(1,n) = n+2\), where \(A\) is the Ackermann function.}

\begin{proof}
1. Basis, for \(n = 1\)
\begin{align*}
    A(1,1) & = A(0,A(1,0))\\
    & = A(0, A(0,1))\\
	& = A(0,2)\\
	& = 3
\end{align*}
Let \(j\) be any natural numbewr greater than 1, that has this property.\\
\begin{align*}
A(1,j) & = j + 2\\
& = A(1,,j+1) \tag*{by induction}\\
& = A(0, A(1,j)) = A(1,j) + 1 \tag*{by definition}\\
& = A(i, j)  = j + 2 + 1\\
& = j + 3
\end{align*}
Therefore, since \(j\) has the property, so does \(k\) such that \(k \in \mathbb{N}\) and \(n < j < k\).
\end{proof}

\end{document}